Update gcd example

test-suite/gcd.v
@@ -1,73 +1,32 @@
 From Equations Require Import Equations.
 Require Import Relations.
-
-Definition gcd_order (p : nat * nat) : nat := let (x,y) := p in x+y.
-
-
-Definition measure {A B} (f : A -> B) (R : relation B) : relation A :=
-  fun x y => R (f x) (f y).
-
-Definition gcd_rel : relation (nat * nat) :=
-  MR lt gcd_order.
-
-Instance gt_bound_wf : WellFounded gcd_rel.
-Proof. red. apply measure_wf. apply Wf_nat.lt_wf. Defined.
-
 Require Import Omega.
 
-Ltac subst_all :=
+Ltac subst_lets :=
   repeat match goal with
   | id := _ |- _ => subst id
   end.
+
 Hint Extern 5 => 
-  unfold gcd_rel, gcd_order, MR; simpl; subst_all; omega : Below.
+  unfold MR; simpl; subst_lets; omega : Below.
 
 Obligation Tactic := program_simpl; try typeclasses eauto with Below.
 
-Equations gcd (p : nat * nat) : nat by wf p gcd_rel :=
-gcd (pair 0 _) := 0 ;
-gcd (pair _ 0) := 0 ;
-gcd (pair (S x) (S y)) with gt_eq_gt_dec x y := {
-  | inleft (left ygtx) := gcd (S x, y - x) ;
-  | inleft (right refl) := S x ;
-  | inright xgty := gcd (x - y, S y) }.
-
-Equations gcd' (p : nat * nat) : nat
-  by wf p gcd_rel :=
-gcd' (pair 0 _) := 0 ;
-gcd' (pair _ 0) := 0 ;
-gcd' (pair x y) with gt_eq_gt_dec x y := {
-  | inleft (left ygtx) := gcd' (x, y - x) ;
+Equations gcd (x y : nat) : nat by wf (x + y) lt :=
+gcd 0 _ := 0 ;
+gcd _ 0 := 0 ;
+gcd x y with gt_eq_gt_dec x y := {
+  | inleft (left ygtx) := gcd x (y - x) ;
   | inleft (right refl) := x ;
-  | inright xgty := gcd' (x - y, y) }.
+  | inright xgty := gcd (x - y) y }.
+Transparent gcd.
+Eval compute in gcd 18 84.
 
 Require Import ExtrOcamlBasic.
 (* Extraction gcd. *)
 (* Extraction gcd_unfold. *)
 
-Lemma gcd_ref x : gcd (x,x) = x.
+Lemma gcd_ref x : gcd x x = x.
 Proof.
-  funelim (gcd (x, x)); now (try (exfalso; omega)). 
+  funelim (gcd x x); now (try (exfalso; omega)).
 Qed.
-
-(* Module Function.     *)
-(* Require Import Recdef. *)
-(* Function gcd (p : nat * nat) {measure gcd_order p} : nat := *)
-(*  match p with *)
-(*    | (0,_) => 0 *)
-(*    | (_,0) => 0 *)
-(*    | (x,y) => match gt_eq_gt_dec x y with *)
-(*                 | inleft (left _) => gcd (x, y-x) *)
-(*                 | inleft (right _) => x *)
-(*                 | inright xgty => gcd (x-y, y) *)
-(*               end *)
-(*  end. *)
-(* - unfold gcd_order ; intros ; omega. *)
-(* - unfold gcd_order ; intros ; omega. *)
-(* Defined. *)
-
-(* Lemma gcd_ref x : gcd (x,x) = x. *)
-(* Proof. *)
-(*   functional induction (gcd (x, x)). Abort. *)
-
-(* End Function. *)
